about to vastly simplify LeafFillDpkv

lib/Buckets/KMBPKVOps.i.dfy
@@ -11,41 +11,105 @@ module KMBPKVOps {
   import DPKV = DynamicPkv
   import KeyType
   import ValueType = ValueType`Internal
+  import opened Sequences
 
-  method FillDpkv(node: KMB.Node, dpkv: DPKV.DynamicPkv)
+  function MessageSeq_to_bytestringSeq(msgs: seq<KMB.Model.Messages.Message>) : (result: seq<seq<byte>>)
+    requires forall i | 0 <= i < |msgs| :: msgs[i].Define?
+    ensures |result| == |msgs|
+    ensures forall i | 0 <= i < |result| :: result[i] == PKV.Message_to_bytestring(msgs[i])
+  {
+    if |msgs| == 0 then
+      []
+    else
+      MessageSeq_to_bytestringSeq(DropLast(msgs)) + [ PKV.Message_to_bytestring(Last(msgs)) ]
+  }
+  
+  method LeafFillDpkv(node: KMB.Node, dpkv: DPKV.DynamicPkv)
     requires KMB.WF(node)
+    requires node.contents.Leaf?
     requires dpkv.WF()
     requires node.repr !! dpkv.Repr
+    requires forall k | k in KMB.Interpretation(node) :: |k| <= KeyType.MaxLen() as nat
+    requires forall v | v in KMB.Interpretation(node).Values :: v.Define?
+    requires PKV.PSA.psaCanAppendSeq(dpkv.toPkv().keys, KMB.ToSeq(node).0)
+    requires forall i | 0 <= i < |KMB.ToSeq(node).1| :: KMB.ToSeq(node).1[i].Define?
+    requires PKV.PSA.psaCanAppendSeq(dpkv.toPkv().messages, MessageSeq_to_bytestringSeq(KMB.ToSeq(node).1))
     ensures dpkv.WF()
     ensures fresh(dpkv.Repr - old(dpkv.Repr))
+    ensures PKV.IKeys(dpkv.toPkv().keys) == old(PKV.IKeys(dpkv.toPkv().keys)) + KMB.ToSeq(node).0
+    ensures PKV.IMessages(dpkv.toPkv().messages) == old(PKV.IMessages(dpkv.toPkv().messages)) + KMB.ToSeq(node).1
     modifies dpkv.Repr
     decreases node.height
   {
+    var keys := node.contents.keys;
+    var values := node.contents.values;
+    var nkeys := node.contents.nkeys;
+
+    assert KMB.ToSeq(node).0 == keys[..nkeys] by {
+      KMB.reveal_I();
+      KMB.Model.reveal_ToSeq();
+    }
+
+    assert KMB.ToSeq(node).1 == values[..nkeys] by {
+      KMB.reveal_I();
+      KMB.Model.reveal_ToSeq();
+    }        
+
+    ghost var oldpkvkeys := old(PKV.IKeys(dpkv.toPkv().keys));
+    ghost var oldpkvmsgs := old(PKV.IMessages(dpkv.toPkv().messages));
+    ghost var messages := MessageSeq_to_bytestringSeq(values[..nkeys]);
+    
     var i: uint64 := 0;
 
-    if node.contents.Leaf? {
-      while i < node.contents.nkeys
-        invariant i <= node.contents.nkeys
-        invariant dpkv.WF()
-        invariant fresh(dpkv.Repr - old(dpkv.Repr))
-      {
-        assume false;
-        dpkv.Append(node.contents.keys[i], node.contents.values[i]);
-        i := i + 1;
+    assert messages[i..nkeys] == MessageSeq_to_bytestringSeq(KMB.ToSeq(node).1);
+
+    while i < nkeys
+      invariant i <= nkeys
+      invariant dpkv.WF()
+      invariant fresh(dpkv.Repr - old(dpkv.Repr))
+      invariant PKV.IKeys(dpkv.toPkv().keys) ==  oldpkvkeys + keys[..i]
+      invariant PKV.PSA.psaCanAppendSeq(dpkv.toPkv().keys, keys[i..nkeys])
+      invariant PKV.IMessages(dpkv.toPkv().messages) == oldpkvmsgs + values[..i]
+      invariant PKV.PSA.psaCanAppendSeq(dpkv.toPkv().messages, messages[i..nkeys])
+    {
+      assert keys[i] in KMB.Interpretation(node) by {
+        KMB.reveal_I();
+        KMB.Model.reveal_Interpretation();
       }
-    } else {
-      while i < node.contents.nchildren
-        invariant i <= node.contents.nchildren
-        invariant dpkv.WF()
-        invariant fresh(dpkv.Repr - old(dpkv.Repr))
-      {
-        KMB.IOfChild(node, i as int);
-        assert KMB.WFShapeChildren(node.contents.children[..node.contents.nchildren], node.repr, node.height);
-        FillDpkv(node.contents.children[i], dpkv);
-        i := i + 1;
-      }
+      assert keys[i..nkeys] == [ keys[i] ] + keys[i+1..nkeys];
+      PKV.PSA.psaCanAppendSeqAdditive(dpkv.toPkv().keys, [ keys[i] ], keys[i+1..nkeys]);
+      PKV.PSA.psaCanAppendOne(dpkv.toPkv().keys, keys[i]);
+
+      assert messages[i..nkeys] == [ messages[i] ] + messages[i+1..nkeys];
+      PKV.PSA.psaCanAppendSeqAdditive(dpkv.toPkv().messages, [ messages[i] ], messages[i+1..nkeys]);
+      PKV.PSA.psaCanAppendOne(dpkv.toPkv().messages, messages[i]);
+      
+      dpkv.Append(keys[i], node.contents.values[i]);
+      
+      assert keys[..i+1] == keys[..i] + [ keys[i] ];
+      assert messages[..i+1] == messages[..i] + [ messages[i] ];
+      assert values[..i+1] == values[..i] + [ values[i] ];
+      i := i + 1;
+    }
+    assert KMB.Model.ToSeq(KMB.I(node)).0 == keys[..i] by {
+      KMB.reveal_I();
+      KMB.Model.reveal_ToSeq();
     }
   }
+
+  // } else {
+  //   assume false;
+  //   while i < node.contents.nchildren
+  //     invariant i <= node.contents.nchildren
+  //     invariant dpkv.WF()
+  //     invariant fresh(dpkv.Repr - old(dpkv.Repr))
+  //   {
+  //     KMB.IOfChild(node, i as int);
+  //     assert KMB.WFShapeChildren(node.contents.children[..node.contents.nchildren], node.repr, node.height);
+  //     FillDpkv(node.contents.children[i], dpkv);
+  //     i := i + 1;
+  //   }
+  // }
 
   method ToPkv(node: KMB.Node) returns (pkv: DPKV.PKV.Pkv)
     requires KMB.WF(node)
@@ -55,7 +119,7 @@ module KMBPKVOps {
     var nelts: uint64 := KMBBOps.CountElements(node);
     var cap := DPKV.Capacity(nelts as uint32, (nelts * KeyType.MaxLen()) as uint32, (nelts * ValueType.MaxLen()) as uint32);
     var dpkv := new DPKV.DynamicPkv.PreSized(cap);
-    FillDpkv(node, dpkv);
+    //FillDpkv(node, dpkv);
     pkv := dpkv.toPkv();
   }
 
